%% Created by Maple 2015.2, Mac OS X
%% Source Worksheet: C6_NewtonsDividedDifference.mw
%% Generated: Fri Aug 19 13:21:47 JST 2016
\documentclass{article}
\usepackage{maplestd2e}
\def\emptyline{\vspace{12pt}}
\begin{document}
\pagestyle{empty}
\DefineParaStyle{Maple Bullet Item}
\DefineParaStyle{Maple Heading 1}
\DefineParaStyle{Maple Warning}
\DefineParaStyle{Maple Heading 4}
\DefineParaStyle{Maple Heading 2}
\DefineParaStyle{Maple Heading 3}
\DefineParaStyle{Maple Dash Item}
\DefineParaStyle{Maple Error}
\DefineParaStyle{Maple Title}
\DefineParaStyle{Maple Text Output}
\DefineParaStyle{Maple Normal}
\DefineCharStyle{Maple 2D Output}
\DefineCharStyle{Maple 2D Input}
\DefineCharStyle{Maple Maple Input}
\DefineCharStyle{Maple 2D Math}
\DefineCharStyle{Maple Hyperlink}
\section{\textbf{Newton(ニュートン) の差分商}}
\begin{maplegroup}
\begin{mapleinput}
\mapleinline{active}{1d}{restart;

X:=[0,1,3,2];
Y:=[1,2,-2,3];
with(LinearAlgebra):
list1:=[X,Y];
}{}
\end{mapleinput}
\mapleresult
\begin{maplelatex}
\mapleinline{inert}{2d}{X := [0, 1, 3, 2]}{\[\displaystyle X\, := \,[0,1,3,2]\]}
\end{maplelatex}
\mapleresult
\begin{maplelatex}
\mapleinline{inert}{2d}{Y := [1, 2, -2, 3]}{\[\displaystyle Y\, := \,[1,2,-2,3]\]}
\end{maplelatex}
\mapleresult
\begin{maplelatex}
\mapleinline{inert}{2d}{list1 := [[0, 1, 3, 2], [1, 2, -2, 3]]}{\[\displaystyle {\it list1}\, := \,[[0,1,3,2],[1,2,-2,3]]\]}
\end{maplelatex}
\end{maplegroup}
\begin{maplegroup}
\begin{mapleinput}
\mapleinline{active}{1d}{with(plots):
l1p:=pointplot(Transpose(Matrix(list1))):
display(l1p);
}{}
\end{mapleinput}
\mapleresult
\mapleplot{C6_NewtonsDividedDifferenceplot2d1.eps}
\end{maplegroup}
\begin{maplegroup}
\begin{mapleinput}
\mapleinline{active}{1d}{F2:=y0+(x-x0)*f1_01+(x-x0)*(x-x1)*f2_012;
F3:=y0+(x-x0)*f1_01+(x-x0)*(x-x1)*f2_012+(x-x0)*(x-x1)*(x-x2)*f3_0123;
}{}
\end{mapleinput}
\mapleresult
\begin{maplelatex}
\mapleinline{inert}{2d}{F2 := y0+(x-x0)*f1_01+(x-x0)*(x-x1)*f2_012}{\[\displaystyle {\it F2}\, := \,{\it y0}+ \left( x-{\it x0} \right) {\it f1\_01}+ \left( x-{\it x0} \right)  \left( x-{\it x1} \right) {\it f2\_012}\]}
\end{maplelatex}
\mapleresult
\begin{maplelatex}
\mapleinline{inert}{2d}{F3 := y0+(x-x0)*f1_01+(x-x0)*(x-x1)*f2_012+(x-x0)*(x-x1)*(x-x2)*f3_0123}{\[\displaystyle {\it F3}\, := \,{\it y0}+ \left( x-{\it x0} \right) {\it f1\_01}+ \left( x-{\it x0} \right)  \left( x-{\it x1} \right) {\it f2\_012}\\
\mbox{}+ \left( x-{\it x0} \right)  \left( x-{\it x1} \right)  \left( x-{\it x2} \right) {\it f3\_0123}\]}
\end{maplelatex}
\end{maplegroup}
\begin{maplegroup}
\begin{mapleinput}
\mapleinline{active}{1d}{f1_01:=(y1-y0)/(x1-x0);
f1_12:=(y2-y1)/(x2-x1);
f1_23:=(y3-y2)/(x3-x2);
}{}
\end{mapleinput}
\mapleresult
\begin{maplelatex}
\mapleinline{inert}{2d}{f1_01 := (y1-y0)/(x1-x0)}{\[\displaystyle {\it f1\_01}\, := \,{\frac {{\it y1}-{\it y0}}{{\it x1}-{\it x0}}}\]}
\end{maplelatex}
\mapleresult
\begin{maplelatex}
\mapleinline{inert}{2d}{f1_12 := (y2-y1)/(x2-x1)}{\[\displaystyle {\it f1\_12}\, := \,{\frac {{\it y2}-{\it y1}}{{\it x2}-{\it x1}}}\]}
\end{maplelatex}
\mapleresult
\begin{maplelatex}
\mapleinline{inert}{2d}{f1_23 := (y3-y2)/(x3-x2)}{\[\displaystyle {\it f1\_23}\, := \,{\frac {{\it y3}-{\it y2}}{{\it x3}-{\it x2}}}\]}
\end{maplelatex}
\end{maplegroup}
\begin{maplegroup}
\begin{mapleinput}
\mapleinline{active}{1d}{f2_012:=(f1_12-f1_01)/(x2-x0);
f2_123:=(f1_23-f1_12)/(x3-x1);
}{}
\end{mapleinput}
\mapleresult
\begin{maplelatex}
\mapleinline{inert}{2d}{f2_012 := ((y2-y1)/(x2-x1)-(y1-y0)/(x1-x0))/(x2-x0)}{\[\displaystyle {\it f2\_012}\, := \,{\frac {1}{{\it x2}-{\it x0}} \left( {\frac {{\it y2}-{\it y1}}{{\it x2}-{\it x1}}}-{\frac {{\it y1}-{\it y0}}{{\it x1}-{\it x0}}}\\
\mbox{} \right) }\]}
\end{maplelatex}
\mapleresult
\begin{maplelatex}
\mapleinline{inert}{2d}{f2_123 := ((y3-y2)/(x3-x2)-(y2-y1)/(x2-x1))/(x3-x1)}{\[\displaystyle {\it f2\_123}\, := \,{\frac {1}{{\it x3}-{\it x1}} \left( {\frac {{\it y3}-{\it y2}}{{\it x3}-{\it x2}}}-{\frac {{\it y2}-{\it y1}}{{\it x2}-{\it x1}}}\\
\mbox{} \right) }\]}
\end{maplelatex}
\end{maplegroup}
\begin{maplegroup}
\begin{mapleinput}
\mapleinline{active}{1d}{f3_0123:=(f2_123-f2_012)/(x3-x0);
}{}
\end{mapleinput}
\mapleresult
\begin{maplelatex}
\mapleinline{inert}{2d}{f3_0123 := (((y3-y2)/(x3-x2)-(y2-y1)/(x2-x1))/(x3-x1)-((y2-y1)/(x2-x1)-(y1-y0)/(x1-x0))/(x2-x0))/(x3-x0)}{\[\displaystyle {\it f3\_0123}\, := \,{\frac {1}{{\it x3}-{\it x0}} \left( {\frac {1}{{\it x3}-{\it x1}} \left( {\frac {{\it y3}-{\it y2}}{{\it x3}-{\it x2}}}-{\frac {{\it y2}-{\it y1}}{{\it x2}-{\it x1}}}\\
\mbox{} \right) }-{\frac {1}{{\it x2}-{\it x0}} \left( {\frac {{\it y2}-{\it y1}}{{\it x2}-{\it x1}}}-{\frac {{\it y1}-{\it y0}}{{\it x1}-{\it x0}}} \right) } \right) }\]}
\end{maplelatex}
\end{maplegroup}
\begin{maplegroup}
\begin{mapleinput}
\mapleinline{active}{1d}{F2;
}{}
\end{mapleinput}
\mapleresult
\begin{maplelatex}
\mapleinline{inert}{2d}{y0+(x-x0)*(y1-y0)/(x1-x0)+(x-x0)*(x-x1)*((y2-y1)/(x2-x1)-(y1-y0)/(x1-x0))/(x2-x0)}{\[\displaystyle {\it y0}+{\frac { \left( x-{\it x0} \right)  \left( {\it y1}-{\it y0} \right) }{{\it x1}-{\it x0}}}+{\frac { \left( x-{\it x0} \right)  \left( x-{\it x1} \right) }{{\it x2}-{\it x0}} \left( {\frac {{\it y2}-{\it y1}}{{\it x2}-{\it x1}}}-{\frac {{\it y1}-{\it y0}}{{\it x1}-{\it x0}}} \right) }\]}
\end{maplelatex}
\end{maplegroup}
\begin{maplegroup}
\begin{mapleinput}
\mapleinline{active}{1d}{for i from 1 to 4 do
  x||(i-1):=X[i];
  y||(i-1):=Y[i];
end:
}{}
\end{mapleinput}
\end{maplegroup}
\begin{maplegroup}
\begin{mapleinput}
\mapleinline{active}{1d}{F2;
F3;
}{}
\end{mapleinput}
\mapleresult
\begin{maplelatex}
\mapleinline{inert}{2d}{1+x-x*(x-1)}{\[\displaystyle 1+x-x \left( x-1 \right) \]}
\end{maplelatex}
\mapleresult
\begin{maplelatex}
\mapleinline{inert}{2d}{1+x-x*(x-1)-x*(x-1)*(x-3)}{\[\displaystyle 1+x-x \left( x-1 \right) -x \left( x-1 \right)  \left( x-3 \right) \]}
\end{maplelatex}
\end{maplegroup}
\begin{maplegroup}
\begin{mapleinput}
\mapleinline{active}{1d}{eq2:=expand(F2);
eq3:=expand(F3);
}{}
\end{mapleinput}
\mapleresult
\begin{maplelatex}
\mapleinline{inert}{2d}{eq2 := -x^2+2*x+1}{\[\displaystyle {\it eq2}\, := \,-{x}^{2}+2\,x+1\]}
\end{maplelatex}
\mapleresult
\begin{maplelatex}
\mapleinline{inert}{2d}{eq3 := -x^3+3*x^2-x+1}{\[\displaystyle {\it eq3}\, := \,-{x}^{3}+3\,{x}^{2}-x+1\]}
\end{maplelatex}
\end{maplegroup}
\begin{maplegroup}
\begin{mapleinput}
\mapleinline{active}{1d}{with(plots):
l1p:=pointplot(Transpose(Matrix(list1))):
pf2:=plot(eq2,x=0..3,color=blue):
pf3:=plot(eq3,x=0..3):
display(l1p,pf2,pf3);
}{}
\end{mapleinput}
\mapleresult
\mapleplot{C6_NewtonsDividedDifferenceplot2d2.eps}
\end{maplegroup}
\begin{maplegroup}
\begin{mapleinput}
\mapleinline{active}{1d}{}{}
\end{mapleinput}
\end{maplegroup}
\end{document}
